First try on the compiling

w39/week_39b_arithmetic_expressions.v
@@ -23,6 +23,15 @@ Inductive arithmetic_expression : Type :=
    Write samples of arithmetic expressions.
 *)
 
+Definition arth_0 :=
+  Lit 5.
+
+Definition arth_1 :=
+  Plus (Lit 4) (Lit 2).
+
+Definition arth_2 :=
+  Plus (Times (Lit 4) (Lit 9)) (Lit 2).
+
 (* ********** *)
 
 Definition specification_of_interpret (interpret : arithmetic_expression -> nat) :=
@@ -39,11 +48,30 @@ Definition specification_of_interpret (interpret : arithmetic_expression -> nat)
    Write unit tests.
 *)
 
+Notation "A =n= B" := (beq_nat A B) (at level 70, right associativity).
+
+Definition unit_test_for_arithmetic_expression (interpret : arithmetic_expression -> nat) :=
+  (interpret arth_0 =n= 5)
+  &&
+  (interpret arth_1 =n= 6)
+  &&
+  (interpret arth_2 =n= 38)
+  .
+
 (* Exercise 2:
    Define an interpreter as a function
    that satisfies the specification above
    and verify that it passes the unit tests.
 *)
+
+Fixpoint interpret_arithmetic (exp : arithmetic_expression) : nat :=
+  match exp with
+    | Lit n => n
+    | Plus a b => interpret_arithmetic a + interpret_arithmetic b
+    | Times a b => interpret_arithmetic a * interpret_arithmetic b
+  end.
+
+Compute unit_test_for_arithmetic_expression interpret_arithmetic.
 
 (* Byte-code instructions: *)
 
@@ -79,7 +107,96 @@ Definition data_stack := list nat.
      from s and then pushing the result of multiplying them.
 
    For now, if the stack underflows, just assume it contains zeroes.
-*)
+ *)
+
+Fixpoint f_on_stack (f : nat -> nat -> nat) (l : data_stack) :=
+  match l with
+    | nil => 0 :: nil
+    | a :: y => 
+      match y with
+        | nil => (f a 0) :: nil
+        | b :: x => (f a b) :: x
+      end
+  end.
+
+Lemma unfold_f_on_stack_zero :
+  (forall f : nat -> nat -> nat,
+  f_on_stack f nil = 0 :: nil).
+Proof.
+  unfold_tactic f_on_stack.
+Qed.
+
+Lemma unfold_f_on_stack_one :
+  (forall (f : nat -> nat -> nat) (n : nat),
+  f_on_stack f (n :: nil) = (f n 0) :: nil).
+Proof.
+  unfold_tactic f_on_stack.
+Qed.
+
+Lemma unfold_f_on_stack_two :
+  (forall (f : nat -> nat -> nat) (x y : nat) (xy : list nat),
+  f_on_stack f (x :: y :: xy) = (f x y) :: xy).
+Proof.
+  unfold_tactic f_on_stack.
+Qed.
+
+Definition specification_of_execute_byte_code_instruction
+           (instr : byte_code_instruction -> data_stack -> data_stack) :=
+  (forall (n : nat) (s : data_stack),
+     instr (PUSH n) s = n :: s)
+  /\
+  (forall (s : data_stack),
+     instr ADD s = (f_on_stack plus s))
+  /\
+  (forall (s : data_stack),
+     instr MUL s = (f_on_stack mult s))
+.
+
+Fixpoint execute_byte_code_instruction (inst : byte_code_instruction) (s : data_stack): data_stack :=
+    match inst with
+      | PUSH n => n :: s
+      | ADD => f_on_stack plus s
+      | MUL => f_on_stack mult s
+  end.
+
+Lemma unfold_execute_byte_code_instruction_push :
+  forall (n : nat) (s : data_stack),
+    execute_byte_code_instruction (PUSH n) s = n :: s.
+Proof.
+  unfold_tactic execute_byte_code_instruction.
+Qed.
+
+Lemma unfold_execute_byte_code_instruction_add :
+  forall (s : data_stack),
+    execute_byte_code_instruction ADD s = f_on_stack plus s.
+Proof.
+  unfold_tactic execute_byte_code_instruction.
+Qed.
+
+Lemma unfold_execute_byte_code_instruction_mul :
+  forall (s : data_stack),
+    execute_byte_code_instruction MUL s = f_on_stack mult s.
+Proof.
+  unfold_tactic execute_byte_code_instruction.
+Qed.
+
+Proposition execute_byte_code_instruction_fits_the_specification_of_execute_byte_code_instruction :
+  specification_of_execute_byte_code_instruction execute_byte_code_instruction.
+Proof.
+  unfold specification_of_execute_byte_code_instruction.
+  unfold execute_byte_code_instruction.
+  split.
+
+  intros n s.
+  reflexivity.
+
+  split.
+  intro s.
+  reflexivity.
+
+  intro s.
+  reflexivity.
+Qed.
 
 (* ********** *)
 
@@ -90,6 +207,27 @@ Definition data_stack := list nat.
    and returns this stack after the program is executed.
 *)
 
+Fixpoint execute_byte_code_program (prog : byte_code_program) (s : data_stack): data_stack :=
+  match prog with
+    | nil => s
+    | x :: y => (execute_byte_code_program y (execute_byte_code_instruction x s))
+  end.
+
+Lemma unfold_execute_byte_code_program_bc :
+  forall (s : data_stack),
+    (execute_byte_code_program nil s) = s.
+Proof.
+  unfold_tactic execute_byte_code_program.
+Qed.
+
+Lemma unfold_execute_byte_code_program_ic :
+  forall (x : byte_code_instruction) (xs : byte_code_program) (s : data_stack),
+    (execute_byte_code_program (x :: xs) s) = (execute_byte_code_program xs (execute_byte_code_instruction x s)).
+Proof.
+  unfold_tactic execute_byte_code_program.
+Qed.
+
+
 (* ********** *)
 
 (* Exercise 5:
@@ -99,6 +237,41 @@ Definition data_stack := list nat.
    (1) executing p1 with s, and then
    (2) executing p2 with the resulting stack.
 *)
+
+Lemma unfold_append_bc :
+  forall (bcis : list byte_code_instruction),
+    nil ++ bcis = bcis.
+Proof.
+  apply app_nil_l.
+Qed.
+
+Lemma unfold_append_ic :
+  forall (bci1 : byte_code_instruction) (bci1s' bci2s : list byte_code_instruction),
+    (bci1 :: bci1s') ++ bci2s = bci1 :: (bci1s' ++ bci2s).
+Proof.
+  intros bci1 bci1s' bci2s.
+  symmetry.
+  apply app_comm_cons.
+Qed.
+
+Theorem append_before_execute_yields_same_result :
+  (forall (p1 p2 : byte_code_program) (s : data_stack),
+     (execute_byte_code_program (p1 ++ p2) s) =
+     (execute_byte_code_program p2 (execute_byte_code_program p1 s))).
+Proof.
+  intro p1.
+  induction p1 as [| x xs IHx].
+    intros p2 s.
+    rewrite -> unfold_execute_byte_code_program_bc.
+    rewrite -> app_nil_l.
+    reflexivity.
+  intros p2 s.
+  rewrite -> unfold_append_ic.
+  rewrite -> (unfold_execute_byte_code_program_ic x (xs ++ p2) s).
+  rewrite -> IHx.
+  rewrite -> unfold_execute_byte_code_program_ic.
+  reflexivity.
+Qed.
 
 (* ********** *)
 
@@ -118,11 +291,169 @@ Definition specification_of_compile (compile : arithmetic_expression -> byte_cod
    and uses list concatenation, i.e., ++.
 *)
 
+Fixpoint compile_expression_v0 (exp : arithmetic_expression) : byte_code_program :=
+  match exp with
+  | Lit n => PUSH n :: nil
+  | Plus ae1 ae2 => compile_expression_v0 ae1 ++ compile_expression_v0 ae2 ++ ADD :: nil
+  | Times ae1 ae2 => compile_expression_v0 ae1 ++ compile_expression_v0 ae2 ++ MUL :: nil
+  end.
+
+Lemma unfold_compile_expression_lit :
+  forall n : nat,
+    compile_expression_v0 (Lit n) = PUSH n :: nil.
+Proof.
+  unfold_tactic compile_expression_v0.
+Qed.
+
+Lemma unfold_compile_expression_plus :
+  forall ae1 ae2 : arithmetic_expression,
+    compile_expression_v0 (Plus ae1 ae2) = compile_expression_v0 ae1 ++ compile_expression_v0 ae2 ++ ADD :: nil.
+Proof.
+  unfold_tactic compile_expression_v0.
+Qed.
+
+Lemma unfold_compile_expression_times :
+  forall ae1 ae2 : arithmetic_expression,
+    compile_expression_v0 (Times ae1 ae2) = compile_expression_v0 ae1 ++ compile_expression_v0 ae2 ++ MUL :: nil.
+Proof.
+  unfold_tactic compile_expression_v0.
+Qed.
+
+
+Proposition compile_expression_v0_fits_the_specification_of_compile :
+  specification_of_compile compile_expression_v0.
+Proof.
+  unfold specification_of_compile.
+  split.
+    exact unfold_compile_expression_lit.
+  split.
+    exact unfold_compile_expression_plus.
+  exact unfold_compile_expression_times.
+Qed.
+
 (* Exercise 7:
    Write a compiler as a function with an accumulator
    that does not use ++ but :: instead,
    and prove it equivalent to the compiler of Exercise 6.
 *)
+
+Fixpoint compile_expression_acc (exp : arithmetic_expression) (prog : byte_code_program) : byte_code_program :=
+  match exp with
+  | Lit n => PUSH n :: prog
+  | Plus ae1 ae2 => (compile_expression_acc ae1 (compile_expression_acc ae2 (ADD :: prog)))  
+  | Times ae1 ae2 => (compile_expression_acc ae1 (compile_expression_acc ae2 (MUL :: prog)))
+  end.
+    
+Lemma unfold_compile_expression_acc_lit :
+  forall (n : nat) (prog : byte_code_program),
+    compile_expression_acc (Lit n) prog = PUSH n :: prog.
+Proof.
+  unfold_tactic compile_expression_acc.
+Qed.
+
+Lemma unfold_compile_expression_acc_plus :
+  forall (ae1 ae2 : arithmetic_expression) (prog : byte_code_program),
+    compile_expression_acc (Plus ae1 ae2) prog = (compile_expression_acc ae1 (compile_expression_acc ae2 (ADD :: prog))).
+Proof.
+  unfold_tactic compile_expression_acc.
+Qed.
+
+Lemma unfold_compile_expression_acc_times :
+  forall (ae1 ae2 : arithmetic_expression) (prog : byte_code_program),
+    compile_expression_acc (Times ae1 ae2) prog = (compile_expression_acc ae1 (compile_expression_acc ae2 (MUL :: prog))).
+Proof.
+  unfold_tactic compile_expression_acc.
+Qed.
+
+Definition compile_expression_v1 (exp : arithmetic_expression) : byte_code_program :=
+  compile_expression_acc exp nil.
+
+Lemma about_compile_expression_acc :
+  forall (exp : arithmetic_expression) (prog : byte_code_program),
+    compile_expression_acc exp prog = compile_expression_acc exp nil ++ prog.
+Proof.
+  intros exp.
+  induction exp as [ | exp1' IHexp1' exp2' IHexp2' | exp1'' IHexp1'' exp2'' IHexp2'' ].
+      intro prog.
+      rewrite ->2 unfold_compile_expression_acc_lit.
+      rewrite -> unfold_append_ic.
+      rewrite -> app_nil_l.
+      reflexivity.
+    intro prog.
+    rewrite ->2 unfold_compile_expression_acc_plus.
+    rewrite -> IHexp1'.
+    rewrite -> IHexp2'.
+    rewrite -> (IHexp1' (compile_expression_acc exp2' (ADD :: nil))).
+    rewrite -> (IHexp2' (ADD :: nil)).
+    rewrite -> app_assoc_reverse.
+    rewrite -> app_assoc_reverse.
+    rewrite -> unfold_append_ic.
+    rewrite -> app_nil_l.
+    reflexivity.
+  intro prog.  
+  rewrite ->2 unfold_compile_expression_acc_times.
+  rewrite -> IHexp1''.
+  rewrite -> IHexp2''.
+  rewrite -> (IHexp1'' (compile_expression_acc exp2'' (MUL :: nil))).
+  rewrite -> (IHexp2'' (MUL :: nil)).
+  rewrite -> app_assoc_reverse.
+  rewrite -> app_assoc_reverse.
+  rewrite -> unfold_append_ic.
+  rewrite -> app_nil_l.
+  reflexivity.
+Qed.
+
+Proposition compile_expression_v1_fits_the_specification_of_compile :
+  specification_of_compile compile_expression_v1.
+Proof.
+  unfold specification_of_compile.
+  split.
+    intro n.
+    unfold compile_expression_v1.
+    rewrite -> unfold_compile_expression_acc_lit.
+    reflexivity.
+  split.
+    intros ae1 ae2.
+    unfold compile_expression_v1.
+    rewrite -> unfold_compile_expression_acc_plus.
+    rewrite -> about_compile_expression_acc.
+    rewrite -> (about_compile_expression_acc ae2 (ADD :: nil)).
+    reflexivity.
+  intros ae1 ae2.
+  unfold compile_expression_v1.
+  rewrite -> unfold_compile_expression_acc_times.
+  rewrite -> about_compile_expression_acc.
+  rewrite -> (about_compile_expression_acc ae2 (MUL :: nil)).
+  reflexivity.
+Qed.
+
+Theorem there_is_only_one_compile_expression :
+  forall (compiler1 compiler2 : arithmetic_expression -> byte_code_program),
+    specification_of_compile compiler1 ->
+    specification_of_compile compiler2 ->
+    forall (exp : arithmetic_expression),
+      compiler1 exp = compiler2 exp.
+Proof.
+  intros compiler1 compiler2.
+  unfold specification_of_compile.
+  intros [H_c1_lit [H_c1_plus H_c1_times]].
+  intros [H_c2_lit [H_c2_plus H_c2_times]].
+  intro exp.
+  induction exp as [ | exp1' IHexp1' exp2' IHexp2' | exp1'' IHexp1'' exp2'' IHexp2'' ].
+      rewrite -> H_c1_lit.
+      rewrite -> H_c2_lit.
+      reflexivity.
+    rewrite -> H_c1_plus.
+    rewrite -> H_c2_plus.
+    rewrite -> IHexp1'.
+    rewrite -> IHexp2'.
+    reflexivity.
+  rewrite -> H_c1_times.
+  rewrite -> H_c2_times.
+  rewrite -> IHexp1''.
+  rewrite -> IHexp2''.
+  reflexivity.
+Qed.
 
 (* ********** *)
 
@@ -131,6 +462,82 @@ Definition specification_of_compile (compile : arithmetic_expression -> byte_cod
    as first compiling it and then executing the compiled program
    over an empty data stack.
 *)
+
+Definition run (prog : byte_code_program) : nat :=
+  match execute_byte_code_program prog nil with
+  | nil => 0
+  | result :: _ => result
+  end.
+
+Lemma unfold_interpret_lit :
+  forall n : nat,
+    interpret_arithmetic (Lit n) = n.
+Proof.
+  unfold_tactic interpret_arithmetic.
+Qed.
+
+Lemma unfold_interpret_plus :
+  forall a b : arithmetic_expression,
+    interpret_arithmetic (Plus a b) = interpret_arithmetic a + interpret_arithmetic b.
+Proof.
+  unfold_tactic interpret_arithmetic.
+Qed.
+
+Lemma unfold_interpret_times :
+  forall a b : arithmetic_expression,
+    interpret_arithmetic (Times a b) = interpret_arithmetic a * interpret_arithmetic b.
+Proof.
+  unfold_tactic interpret_arithmetic.
+Qed.
+
+Lemma interpret_cons_datastack_eq_compile_execute :
+  forall (exp : arithmetic_expression) (ds : data_stack),
+    interpret_arithmetic exp :: ds = execute_byte_code_program (compile_expression_v0 exp) ds.
+Proof.
+  intro exp.
+  induction exp as [ n | exp1' IHexp1' exp2' IHexp2' | exp1'' IHexp1'' exp2'' IHexp2''].
+      intro ds.
+      rewrite -> unfold_interpret_lit.
+      rewrite -> unfold_compile_expression_lit.
+      rewrite -> unfold_execute_byte_code_program_ic.
+      rewrite -> unfold_execute_byte_code_instruction_push.
+      rewrite -> unfold_execute_byte_code_program_bc.
+      reflexivity.
+    intro ds.
+    rewrite -> unfold_interpret_plus.
+    rewrite -> unfold_compile_expression_plus.
+    rewrite ->2 append_before_execute_yields_same_result.
+    rewrite -> unfold_execute_byte_code_program_ic.
+    rewrite -> unfold_execute_byte_code_instruction_add.
+    rewrite -> unfold_execute_byte_code_program_bc.
+    rewrite <- IHexp1'.
+    rewrite <- IHexp2'.
+    rewrite -> unfold_f_on_stack_two.
+    rewrite -> plus_comm.
+    reflexivity.
+  intro ds.
+  rewrite -> unfold_interpret_times.
+  rewrite -> unfold_compile_expression_times.
+  rewrite ->2 append_before_execute_yields_same_result.
+  rewrite -> unfold_execute_byte_code_program_ic.
+  rewrite -> unfold_execute_byte_code_instruction_mul.
+  rewrite -> unfold_execute_byte_code_program_bc.
+  rewrite <- IHexp1''.
+  rewrite <- IHexp2''.
+  rewrite -> unfold_f_on_stack_two.
+  rewrite -> mult_comm.
+  reflexivity.
+Qed.
+
+Theorem interpret_exp_eq_run_compile_exp :
+  forall (exp : arithmetic_expression),
+    interpret_arithmetic exp = run (compile_expression_v0 exp).
+Proof.
+  intro exp.
+  unfold run.
+  rewrite <- interpret_cons_datastack_eq_compile_execute.
+  reflexivity.
+Qed.
 
 (* ********** *)
 
@@ -158,11 +565,158 @@ Definition specification_of_compile (compile : arithmetic_expression -> byte_cod
 
 *)
 
+Definition data_stack2 := list arithmetic_expression.
+
+Fixpoint magritte_v0 (prog : byte_code_program) (s : data_stack2) :=
+  match prog with
+  | nil => s
+  | (PUSH n) :: prog' => magritte_v0 prog' ((Lit n) :: s)
+  | ADD :: prog' => 
+      match s with
+      | nil => magritte_v0 prog' ((Plus (Lit 0) (Lit 0)) :: nil)
+      | exp :: nil => magritte_v0 prog' ((Plus (Lit 0) exp) :: nil)
+      | exp1 :: exp2 :: exps => magritte_v0 prog' ((Plus exp2 exp1) :: exps)
+      end
+  | MUL :: prog' => 
+      match s with
+      | nil => magritte_v0 prog' ((Times (Lit 0) (Lit 0)) :: nil)
+      | exp :: nil => magritte_v0 prog' ((Times (Lit 0) exp) :: nil)
+      | exp1 :: exp2 :: exps => magritte_v0 prog' ((Times exp2 exp1) :: exps)
+      end
+  end.
+
+Lemma unfold_magritte_v0_nil_prog :
+  forall (s : data_stack2),
+    magritte_v0 nil s = s.
+Proof.
+  unfold_tactic magritte_v0.
+Qed.
+
+Lemma unfold_magritte_v0_push :
+  forall (n : nat) (prog' : byte_code_program) (s : data_stack2),
+    magritte_v0 ((PUSH n) :: prog') s = magritte_v0 prog' ((Lit n) :: s).
+Proof.
+  unfold_tactic magritte_v0.
+Qed.
+
+Lemma unfold_magritte_v0_add_nil :
+  forall (prog' : byte_code_program) (s : data_stack2),
+    magritte_v0 (ADD :: prog') nil = magritte_v0 prog' ((Plus (Lit 0) (Lit 0)) :: nil).
+Proof.
+  unfold_tactic magritte_v0.
+Qed.
+
+Lemma unfold_magritte_v0_add_1 :
+  forall (prog' : byte_code_program) (exp : arithmetic_expression) (s : data_stack2),
+    magritte_v0 (ADD :: prog') (exp :: nil) = magritte_v0 prog' ((Plus (Lit 0) exp) :: nil).
+Proof.
+  unfold_tactic magritte_v0.
+Qed.
+
+Lemma unfold_magritte_v0_add_2 :
+  forall (prog' : byte_code_program) (exp1 exp2 : arithmetic_expression) (s : data_stack2),
+    magritte_v0 (ADD :: prog') (exp1 :: exp2 :: s) = magritte_v0 prog' ((Plus exp2 exp1) :: s).
+Proof.
+  unfold_tactic magritte_v0.
+Qed.
+
+Lemma unfold_magritte_v0_mul_nil :
+  forall (prog' : byte_code_program) (s : data_stack2),
+    magritte_v0 (MUL :: prog') nil = magritte_v0 prog' ((Times (Lit 0) (Lit 0)) :: nil).
+Proof.
+  unfold_tactic magritte_v0.
+Qed.
+
+Lemma unfold_magritte_v0_mul_1 :
+  forall (prog' : byte_code_program) (exp : arithmetic_expression) (s : data_stack2),
+    magritte_v0 (MUL :: prog') (exp :: nil) = magritte_v0 prog' ((Times (Lit 0) exp) :: nil).
+Proof.
+  unfold_tactic magritte_v0.
+Qed.
+
+Lemma unfold_magritte_v0_mul_2 :
+  forall (prog' : byte_code_program) (exp1 exp2 : arithmetic_expression) (s : data_stack2),
+    magritte_v0 (MUL :: prog') (exp1 :: exp2 :: s) = magritte_v0 prog' ((Times exp2 exp1) :: s).
+Proof.
+  unfold_tactic magritte_v0.
+Qed.
+
+Definition run_magritte (prog : byte_code_program) : arithmetic_expression :=
+  match (magritte_v0 prog nil) with
+  | nil => Lit 0
+  | exp :: _ => exp
+  end.
+
+Compute arth_2.
+Compute compile_expression_v0 arth_2.
+Compute run_magritte (compile_expression_v0 arth_2).
+
 (* Exercise 10:
    Prove that the Magrite-style execution function from Exercise 9
    implements a decompiler that is the left inverse of the compiler
    of Exercise 6.
 *)
+
+Lemma append_before_magritte_yields_same_result :
+  forall (p1 p2 : byte_code_program) (s : data_stack2),
+       magritte_v0 (p1 ++ p2) s =
+       magritte_v0 p2 (magritte_v0 p1 s).
+Proof.
+  intro p1.
+  induction p1 as [ | x xs' IHxs'].
+    intros p2 s.
+    rewrite -> unfold_magritte_v0_nil_prog.
+    rewrite -> app_nil_l.
+    reflexivity.
+  intros p2 s.
+  Check unfold_append_ic.
+  rewrite -> unfold_append_ic.
+  induction x.
+      rewrite ->2 unfold_magritte_v0_push.
+      rewrite -> IHxs'.
+      reflexivity.
+    induction s.
+    rewrite ->2 unfold_magritte_v0_add_nil.
+    rewrite ->2 unfold_magritte_v0_add_1.
+
+Lemma exp_cons_exps_eq_magritte_compile_exp :
+  forall (exp : arithmetic_expression) (s : data_stack2),
+    exp :: s = magritte_v0 (compile_expression_v0 exp) s.
+Proof.
+  intro exp.
+  induction exp as [ | exp1' IHexp1' exp2' IHexp2' | exp1'' IHexp1'' exp2'' IHexp2''].
+      intro s.
+      rewrite -> unfold_compile_expression_lit.
+      rewrite -> unfold_magritte_v0_push.
+      rewrite -> unfold_magritte_v0_nil_prog.
+      reflexivity.
+    intro s.
+    rewrite -> unfold_compile_expression_plus.
+    rewrite ->2 append_before_magritte_yields_same_result.
+    rewrite <- IHexp1'.
+    rewrite <- IHexp2'.
+    rewrite -> unfold_magritte_v0_add_2.
+    rewrite -> unfold_magritte_v0_nil_prog.
+    reflexivity.
+  intro s.
+  rewrite -> unfold_compile_expression_times.
+  rewrite ->2 append_before_magritte_yields_same_result.
+  rewrite <- IHexp1''.
+  rewrite <- IHexp2''.
+  rewrite -> unfold_magritte_v0_mul_2.
+  rewrite -> unfold_magritte_v0_nil_prog.
+  reflexivity.
+Qed.
+
+Theorem compile_exp_and_run_magritte_gives_exp :
+  forall exp : arithmetic_expression,
+    exp = run_magritte (compile_expression_v0 exp).
+Proof.
+  intro exp.
+  unfold run_magritte.
+  rewrite <- exp_cons_exps_eq_magritte_compile_exp.
+  reflexivity.
+Qed.
 
 (* ********** *)
 
